src/3d/Binding.fst
@@ -331,7 +331,7 @@ let typ_is_integral env (t:typ) : ML bool =
 
 let tag_of_integral_typ env (t:typ) : ML (option _) =
   match t.v with
-  | Pointer _ (PQ a) -> Some a
+  | Pointer _ pq -> Some <| pq_as_integer_type pq
   | Type_app hd _ _ _ -> (
     match lookup env hd with
     | Inr (_, Inl attrs) -> attrs.integral
@@ -341,7 +341,7 @@ let tag_of_integral_typ env (t:typ) : ML (option _) =
 
 let tag_and_bit_order_of_integral_typ env (t:typ) : ML (tag_and_bit_order: (option integer_type & option bitfield_bit_order) { Some? (snd tag_and_bit_order) ==> Some? (fst tag_and_bit_order) }) =
   match t.v with
-  | Pointer _ (PQ a) -> Some a, None
+  | Pointer _ pq -> Some <| pq_as_integer_type pq, None
   | Type_app hd _ _ _ -> (
     match lookup env hd with
     | Inr (_, Inl attrs) -> attrs.integral, attrs.bit_order
@@ -366,7 +366,7 @@ let parser_weak_kind (env:global_env) (id:ident) : ML (option _) =
 
 let rec typ_weak_kind env (t:typ) : ML (option weak_kind) =
   match t.v with
-  | Pointer _ (PQ i) -> typ_weak_kind env (type_of_integer_type i)
+  | Pointer _ pq -> typ_weak_kind env (type_of_integer_type (pq_as_integer_type pq))
   | Type_app hd _ _ _ -> parser_weak_kind env.globals hd
   | _ -> None
 
@@ -631,7 +631,7 @@ let rec check_out_expr (env:env) (oe0:out_expr)
           out_expr_t = oe_t;
           out_expr_bit_width = bopt } = Some?.v oe.out_expr_meta in
     (match oe_t.v, bopt with
-     | Pointer t (PQ UInt64), None ->
+     | Pointer t (PQ UInt64 _), None ->
        {oe0 with
         out_expr_node={oe0.out_expr_node with v=OE_star oe};
         out_expr_meta=Some ({ out_expr_base_t = oe_bt;
@@ -653,7 +653,7 @@ let rec check_out_expr (env:env) (oe0:out_expr)
 
         out_expr_meta=Some ({
           out_expr_base_t = oe_bt;
-          out_expr_t = with_range (Pointer oe_t (PQ UInt64)) oe.out_expr_node.range;
+          out_expr_t = with_range (Pointer oe_t (PQ UInt64 true)) oe.out_expr_node.range;
           out_expr_bit_width = None })}
      | _ ->
        error
@@ -665,7 +665,7 @@ let rec check_out_expr (env:env) (oe0:out_expr)
           out_expr_t = oe_t;
           out_expr_bit_width = bopt }  = Some?.v oe.out_expr_meta in
     (match oe_t.v, bopt with
-     | Pointer t (PQ UInt64), None ->
+     | Pointer t (PQ UInt64 _), None ->
        let i = check_output_type (global_env_of_env env) t in
        let out_expr_t, out_expr_bit_width = lookup_output_type_field
          (global_env_of_env env)
@@ -717,13 +717,7 @@ let rec check_typ (pointer_ok:bool) (env:env) (t:typ)
 
     | Pointer t0 pq ->
       let check_pointer_qualifier : pointer_qualifier -> ML pointer_qualifier =
-        function
-        | PQ a ->
-          match a with
-          | UInt32
-          | UInt64 ->
-            PQ a
-          | _ -> error (Printf.sprintf "Pointer qualifier %s must be either UINT32 or UINT64" (print_integer_type a)) t.range
+        fun p -> p
       in
       if pointer_ok
       then { t with v = Pointer (check_typ pointer_ok env t0) (check_pointer_qualifier pq) }
@@ -1171,7 +1165,7 @@ let rec check_field_action (env:env) (f:atomic_field) (a:action)
           let t = lookup_expr_name env i in
           begin
           match t.v with
-          | Pointer t (PQ UInt64) -> Action_deref i, t
+          | Pointer t (PQ UInt64 _) -> Action_deref i, t
           | _ -> error "Dereferencing a non-pointer" i.range
           end
 
@@ -1272,6 +1266,26 @@ let rec check_probe env a : ML (probe_action & typ) =
     | Probe_action_return e ->
       let e, t= check_expr env e in
       Probe_action_return e, t
+    | Probe_action_init f n -> (
+      let n, t = check_expr env n in
+      let n =
+        match try_cast_integer env (n, t) tuint64 with
+        | None ->
+          error (Printf.sprintf "Probe length value %s has type %s instead of UINT64"
+                    (print_expr n)
+                    (print_typ t))
+                    n.range
+        | Some n ->
+          n
+      in
+      match GlobalEnv.resolve_probe_fn_any env.globals f with
+      | Some (id, Inr (Some PQInit)) ->
+        Probe_action_init f n, tunit
+      | _ ->
+        error (Printf.sprintf "Probe function %s not found or not an init function" (print_ident f))
+              f.range
+    )        
+    
     | Probe_action_skip n ->
       let n, t = check_expr env n in
       if not (eq_typ env t tuint64)
@@ -1498,7 +1512,7 @@ let check_atomic_field (env:env) (extend_scope: bool) (f:atomic_field)
         : ML (option ident)
         = let ptr_size =
             match sf.field_type.v with
-            | Pointer _ (PQ sz) -> sz
+            | Pointer _ pq -> pq_as_integer_type pq
             | _ ->
               error (
                   Printf.sprintf "Probes are only allowed on pointer fields, got %s"
@@ -2015,8 +2029,8 @@ let rec check_mutable_param_type (env:env) (t:typ) : ML typ =
        (i.v.modul_name = None && List.Tot.mem i.v.name allowed_base_types_as_output_types)
     then t
     else err (Some i)
-  | Pointer t (PQ UInt64) -> 
-    { t with v = Pointer (check_mutable_param_type env t) (PQ UInt64) }
+  | Pointer t (PQ UInt64 explicit) -> 
+    { t with v = Pointer (check_mutable_param_type env t) (PQ UInt64 explicit) }
   | _ -> err None
     
 let rec check_integer_or_output_type (env:env) (t:typ) : ML unit =
@@ -2026,7 +2040,7 @@ let rec check_integer_or_output_type (env:env) (t:typ) : ML unit =
     if i.v.modul_name = None && List.Tot.mem i.v.name allowed_base_types_as_output_types
     then ()
     else if not (k = KindOutput) then error (Printf.sprintf "%s is not an integer or output type" (print_typ t)) t.range
-  | Pointer t (PQ UInt64) -> check_integer_or_output_type env t
+  | Pointer t (PQ UInt64 _) -> check_integer_or_output_type env t
   | _ -> error (Printf.sprintf "%s is not an integer or output type" (print_typ t)) t.range
 
 let check_mutable_param (env:env) (p:param) : ML param =
@@ -2034,8 +2048,8 @@ let check_mutable_param (env:env) (p:param) : ML param =
   //and the base type may be a base type or an output type
   let t, i, q = p in
   match t.v with
-  | Pointer bt (PQ UInt64) ->
-    let t = { t with v = Pointer (check_mutable_param_type env bt) (PQ UInt64) } in
+  | Pointer bt (PQ UInt64 explicit) ->
+    let t = { t with v = Pointer (check_mutable_param_type env bt) (PQ UInt64 explicit) } in
     t, i, q 
   | _ ->
     error (Printf.sprintf "%s is not a valid mutable parameter type, it is not a pointer type" (print_typ t)) t.range
